Second test study

Praticas/TP10/selectionSort.dfy
@@ -4,21 +4,44 @@
 */
 
 // Sorts array 'a' using the selection sort algorithm.
-method selectionSort(a: array<real>) {
+method selectionSort(a: array<real>) 
+    modifies a
+    ensures isSorted(a, 0, a.Length)
+    ensures multiset(a[..]) == multiset(old(a[..]))
+{
     var i := 0; 
-    while i < a.Length - 1 {
+    while i < a.Length - 1 
+        invariant 0 <= i <= a.Length
+        invariant isSorted(a, 0, i)
+        invariant multiset(a[..]) == multiset(old(a[..]))
+        invariant forall l, r :: 0 <= l < i <= r < a.Length ==> a[l] <= a[r]
+    {
         var j := findMin(a, i, a.Length); // minimum in remaining subarray
         a[i], a[j] := a[j], a[i]; // swap
         i := i + 1;
     }
 }
 
+predicate isSorted(a: array<real>, from: nat, to: nat)
+    reads a
+    requires 0 <= from <= to <= a.Length
+{   
+    forall i, j :: from <= i < j < to ==> a[i] <= a[j]
+}
+
 // Finds the position of a miminum value in a non-empty subarray 'a' between positions 
 // 'from' (inclusive) and 'to' (exclusive)
-method findMin(a: array<real>, from: nat, to: nat) returns(index: nat) {
+method findMin(a: array<real>, from: nat, to: nat) returns(index: nat) 
+    requires from < to <= a.Length
+    ensures from <= index < to
+    ensures forall i :: from <= i < to ==> a[index] <= a[i]
+{
     var i := from + 1;
     index := from; // position of min up to position i (excluded)
-    while i < to {
+    while i < to 
+        invariant from <= i <= to && from <= index < i
+        invariant forall j :: from <= j < i ==> a[index] <= a[j]
+    {
         if a[i] < a[index] {
             index := i;
         }
