Praticas/TP11/Bank.dfy
@@ -9,26 +9,54 @@ class BankAccount {
     var balance: real;
     
     constructor (initialBalance: real)
+        requires initialBalance >= 0.0
+        ensures Valid()
+        ensures balance == initialBalance
     {
         balance := initialBalance;
     }
+
+    predicate Valid()
+        reads this
+    {
+        balance >= 0.0
+    }
  
     function method getBalance() : real
+        reads this
     {
         balance
     }
 
     method deposit(amount : real)
+        modifies this
+        requires Valid()
+        requires amount >= 0.0
+        ensures balance == old(balance) + amount
+        ensures Valid()
     {
         balance := balance + amount;
     }
 
     method withdraw(amount : real)
+        modifies this
+        requires Valid()
+        requires amount < balance
+        ensures balance == old(balance) - amount
+        ensures Valid()
     {
         balance := balance - amount;
     }
 
     method transfer(amount : real, destination: BankAccount)
+        modifies this
+        modifies destination
+        requires Valid()
+        requires this != destination
+        requires amount <= this.balance
+        ensures destination.balance == old(destination.balance) + amount
+        ensures this.balance == old(this.balance) - amount
+        ensures Valid()
     {
         this.balance := this.balance - amount;
         destination.balance:= destination.balance + amount;
