Praticas/TP11/Figure.dfy
@@ -6,24 +6,25 @@
 trait Figure {
     var center: (real, real);
 
-    predicate Valid()
-      reads this
+    // predicate Valid()
+    //     reads this
       
     function method getSizeX(): real
-       requires Valid()
-       reads this
+        // requires Valid()
+        reads this
 
     function method getSizeY(): real
-       requires Valid()
-       reads this
+        // requires Valid()
+        reads this
     
     method resize(factor: real)
-      requires factor > 0.0 && Valid()
-      modifies this
-      ensures Valid()
-      ensures getSizeX() == factor * old(getSizeX()) 
-      ensures getSizeY() == factor * old(getSizeY())
-      ensures center == old(center) 
+        requires factor > 0.0
+        // requires Valid()
+        modifies this
+        // ensures Valid()
+        ensures getSizeX() == factor * old(getSizeX()) 
+        ensures getSizeY() == factor * old(getSizeY())
+        ensures center == old(center) 
 }
 
 class Circle extends Figure {
@@ -36,16 +37,22 @@ class Circle extends Figure {
     }
     
     function method getSizeX(): real
+        reads this
     {
         radius
     }
 
     function method getSizeY(): real
+        reads this
     {
         radius
     }
 
     method resize(factor: real)
+        modifies this
+        requires factor != 0.0
+        ensures center == old(center)
+        ensures radius == abs(factor) * old(radius)
     {
        radius := abs(factor) * radius;
     }
