Praticas/TP12/ArraySet_Ghost.dfy
@@ -1,0 +1,158 @@
+/* 
+* Specification, implementation and verification of a Set implemented with an array (resizable).
+* Illustrates the usage of ghost variables and abstraction/refinment relations to better separate
+* specification (interface) and implementation.
+* Pre/post-conditions of public operations are defined in terms of the abstract state variables.
+* FEUP, M.EIC, MFS, 2021/22.
+*/
+
+class {:autocontracts} ArraySet<T(==)> {
+  // (Public) ghost variables used for specification purposes only  
+  ghost var elems: set<T>;
+ 
+  // (Private) concrete variables with internal representation.
+  var list: array<T>;
+  var used : nat;
+  const initializer: nat -> T;
+
+  // (Private) predicate that formalizes the class invariant.  
+  predicate Valid() {
+    // constraints on concrete representation
+    used <= list.Length 
+    && list.Length > 0
+    && (forall i, j :: 0 <= i < j < used ==> list[i] != list[j]) // no duplicates
+    // abstraction relation (between concrete and abstract variables)
+    && elems == set x | x in list[..used] 
+  }
+
+  // (Public) Constructor, initializes this set as empty.
+  constructor (initializer: nat -> T)
+    ensures elems == {}
+  {
+    // initialize concrete state variables
+    list := new T[10] (initializer); 
+    used := 0;
+    this.initializer := initializer;
+    // initialize ghost state variable
+    elems := {};
+  }
+
+  // (Public) Checks if this set contains an element x.
+  predicate method contains(x: T) 
+    ensures contains(x) <==> x in elems  
+  {
+    // search concrete state variables
+    exists i :: 0 <= i < used && list[i] == x
+  }
+
+  // (Public) Inserts a new element x into this set.
+  method insert(x : T)
+    requires x !in elems
+    ensures elems == old(elems) + {x}
+  {
+    // allocate larger array if needed
+    if used == list.Length { 
+      grow();
+    }
+    // update concrete variables
+	  list[used] := x;
+    // trick: remind Dafny that other positions were not changed!!
+    assert list[..used] == old(list[..used]);
+    used := used + 1;
+    // update ghost variable
+    elems := elems + {x};
+  }
+
+  // (Private) Auxiliary method to reallocate the array.
+  method grow()
+    ensures list.Length > old(list.Length)
+    ensures list[..used] == old(list[..used])
+  {
+    var oldList := list;
+    list := new T[ 2 * list.Length](initializer);
+    forall i | 0 <= i < used {
+        list[i] := oldList[i];
+    }
+    // trick: remind Dafny thar values were not changed (to prove Valid)
+    assert list[..used] == old(list[..used]);
+  }
+
+  // (Public) Deletes an existing element x from this set in time O(n).
+  method delete(x: T)
+    requires x in elems
+    ensures elems == old(elems) - {x} 
+  {
+    // update concrete variables
+    var i :| 0 <= i < used && list[i] == x;
+    list[i] := list[used-1];
+    // remind Dafny that other positions were not changed!!
+    assert forall j :: 0 <= j < used && j != i ==> list[j] == old(list[j]);
+    used := used-1;
+    // update ghost variable
+    elems := elems - {x};
+  }
+
+  // (Public) Obtains the size of the set
+  function method size(): nat
+    ensures size() == |elems|  
+  {
+    // recalls property to prove the post-condition
+    assert elems == elemsN(used);
+    sizeProp(used);
+    // now return the expression 
+    used
+  }
+
+  // Same as elems, but for a part of the list.
+  function elemsN(n: nat): set<T> 
+     requires n <= used
+  {
+      set x | x in list[..n]
+  }
+  
+  // Proves (by induction on the length (n) of list) that, since the list has no 
+  // duplicates, the size of the corresponding set equals the length of the list. 
+  lemma sizeProp(n: nat)
+   requires n <= used
+   ensures |elemsN(n)| == n
+  {
+    if n > 0 { 
+      // recall the same property for a simpler case (n-1)
+      sizeProp(n-1);
+      // fact needed to complete the proof
+      assert elemsN(n) == elemsN(n-1) + {list[n-1]};
+    }
+  }
+}
+
+// A simple test scenario checked statically.
+method testSet() {
+  var s := new ArraySet<int>(n => 0);
+  s.insert(2);
+  s.insert(5);
+  assert s.size() == 2;
+  assert s.contains(2);
+  assert s.contains(5);
+  assert !s.contains(1);
+  s.delete(2);
+  assert s.size() == 1;
+  assert s.contains(5);
+  assert !s.contains(2);
+  s.delete(5);
+  assert !s.contains(5);
+  assert s.size() == 0;
+}
+
+
+// Examples of test cases with invalid inputs
+// method testInvalidDelete() {
+//   var s := new ArraySet();
+//   s.insert(1);
+//   s.delete(2);
+// }
+
+// method testInvalidInsert() {
+//   var s := new ArraySet();
+//   s.insert(1);
+//   s.insert(1);
+// }
