Testes anteriores/T2/bubble_2018.dfy
@@ -1,0 +1,34 @@
+method bubbleSort(a: array<real>)
+    // ensures forall k :: 0 <= k <= a.Length ==> a[k] <= a[k+1]
+    ensures forall i,j :: 0 <= i < j <= a.Length - 1 ==> a[i] <= a[j]
+    ensures forall i,j :: 0 <= i <= a.Length - 1 && i+1 <= j <= a.Length - 1 ==> a[i] <= a[j]
+    ensures forall k :: 1 <= k <= a.Length - 1 ==> a[k-1] <= a[k]
+{
+    var i : int := a.Length - 1;
+    while (i > 0) 
+        invariant -1 <= i <= a.Length - 1
+    
+    {
+        innerLoop(a, i);
+        i := i - 1;
+    }
+} 
+
+method innerLoop(a: array<real>, i: int) 
+{
+    var j: int := 0;
+    while (j < i)
+        invariant 0 <= j <= i && forall k :: 0 <= k <= j-1 ==> a[k] <= a[j]
+    {
+        if (a[j] > a[j+1]) 
+        {
+            swap(a, j, j+1);
+        }
+        j:= j + 1;
+    }
+}
+
+method swap(a: array<real>, from: int, to: int)
+{
+
+}
