Testes anteriores/T2/deque_ghost.dfy
@@ -1,0 +1,130 @@
+type T = int // for demo purposes, but could be another type
+
+class {:autocontracts} Deque {
+    // (Private) concrete state variables
+    const list: array<T>; // circular array, from list[start] (front) to
+                        // list[(start+size-1) % list.Length] (back)
+    var start : nat;
+    var size : nat;
+
+    // (Public) ghost variables used for specification purposes only
+    ghost var elems: seq<T>; // front at head, back at tail
+    ghost const capacity: nat;
+
+    constructor (capacity: nat) 
+        requires capacity > 0
+        ensures elems == [] && this.capacity == capacity
+        ensures start == 0 && size == 0
+    {
+        list := new T[capacity];
+        start := 0;
+        size := 0;
+
+        this.capacity := capacity;
+        elems := [];
+    }
+
+    predicate Valid()
+        reads this
+    {
+        size <= list.Length &&
+        0 <= start < list.Length &&
+        capacity == list.Length &&
+        if start + size <= list.Length then
+            elems == list[start .. start + size]
+        else
+            elems == list[start..] + list[..(start + size) - list.Length]
+    }
+
+    predicate method isEmpty() 
+        ensures isEmpty() <==> |elems| == 0
+    {
+        size == 0
+    }
+
+    predicate method isFull() 
+        ensures isFull() <==> |elems| == capacity
+    {
+        size == list.Length
+    }
+
+    function method front() : T 
+        requires !isEmpty()
+        ensures front() == elems[0]
+    {
+        list[start]
+    }
+
+    function method back() : T 
+        requires !isEmpty()
+        ensures back() == elems[ |elems| - 1]
+    {
+        list[(start + size - 1) % list.Length]
+    }
+
+    method push_back(x : T) 
+        requires !isFull()
+        ensures elems == old(elems) + [x]
+    {
+        if start + size + 1 <= list.Length {
+            list[start + size] := x;
+        }
+        else {
+            list[start + size - list.Length] := x;
+        }
+        size := size + 1;
+
+        elems := elems + [x];
+    }
+
+    method pop_back() 
+        requires !isEmpty()
+        ensures elems == old(elems[..|elems| - 1])
+    {
+        size := size - 1;
+        elems := elems[..size];
+    }
+
+    method push_front(x : T) 
+        requires !isFull()
+        ensures elems == [x] + old(elems)
+    {
+        start := if start > 0 then start - 1 else list.Length - 1;
+        list[start] := x;
+        size := size + 1;
+        elems := [x] + elems;
+    }
+
+    method pop_front() 
+        requires !isEmpty()
+        ensures elems == old(elems[1..])
+    {
+        start := if start + 1 < list.Length then start + 1 else 0;
+        size := size - 1;
+        elems := elems[1..];
+    }
+}
+// A simple test scenario.
+method testDeque()
+{
+    var q := new Deque(3);
+    assert q.isEmpty();
+    q.push_front(1);
+    assert q.front() == 1;
+    assert q.back() == 1;
+    q.push_front(2);
+    assert q.front() == 2;
+    assert q.back() == 1;
+    q.push_back(3);
+    assert q.front() == 2;
+    assert q.back() == 3;
+    assert q.isFull();
+    q.pop_back();
+    assert q.front() == 2;
+    assert q.back() == 1;
+    q.pop_front();
+    assert q.front() == 1;
+    assert q.back() == 1;
+    q.pop_front();
+    assert q.isEmpty();
+}
