Testes anteriores/T2/div.dfy
@@ -1,0 +1,53 @@
+function method abs(d: int) : nat
+{
+    if d >= 0 then d else -d
+}
+
+function method sign(d : int) : int
+{
+    if d >= 0 then 1 else -1
+}
+
+method div(n: int, d: int) returns (q: int, r: int)
+  requires d != 0
+  ensures 0 <= r < abs(d)
+  ensures q * d + r == n
+{
+  q := 0;
+  r := n;  
+
+  if n > 0
+  {
+    while r >= abs(d)
+        decreases r
+        invariant r >= 0
+        invariant q * d + r == n
+    {
+        q := q + sign(d);
+        r := r - abs(d);
+    }
+  }
+  else if n < 0
+  {
+    while r < 0
+        decreases abs(d) - r
+        invariant r < abs(d) 
+        invariant q * d + r == n
+    {
+        q := q - sign(d);
+        r := r + abs(d);
+    }
+  }
+}
+
+// A simple test case
+method Main()
+{
+  var q, r := div(15, 6);
+  print "q = ", q, " r = ", r, "\n";
+  assert q == 2 && r == 3;
+
+  var q1, r1 := div(15, -6);
+  print "q = ", q1, " r = ", r1, "\n";
+  assert q1 == -2 && r1 == 3;
+}
