Testes anteriores/T2/ex6_2020.dfy
@@ -1,0 +1,56 @@
+type T = int
+
+predicate sorted(a: array<T>, n: nat)
+  reads a
+  requires 0 <= n <= a.Length
+{
+  forall i, j :: 0 <= i < j < n ==> a[i] <= a[j]
+}
+
+function elems(a: array<T>, n: nat): multiset<T>
+  requires n <= a.Length
+  reads a
+{
+  multiset(a[..n])
+}
+
+// Merges two sorted arrays 'a' and 'b' into a new sorted array 'c'
+method merge(a: array<T>, b: array<T>) returns (c: array<T>) 
+    requires sorted(a, a.Length)
+    requires sorted(b, b.Length)
+    ensures sorted(c, c.Length)
+    ensures elems(c, c.Length) == elems(a, a.Length) + elems(b, b.Length)
+{
+    c := new T[a.Length + b.Length];
+    var i, j := 0, 0;
+
+    // Repeatedly pick the smallest element from 'a' and 'b' and copy it into 'c'
+    while i < a.Length || j < b.Length 
+        decreases (a.Length - i) + (b.Length - j)
+        invariant 0 <= i <= a.Length
+        invariant 0 <= j <= b.Length
+        invariant sorted(c, i + j)
+        invariant elems(c, i + j) == elems(a, i) + elems(b, j)
+        invariant forall k, l :: i <= k < a.Length && 0 <= l < i + j ==> a[k] >= c[l]
+        invariant forall k, l :: j <= k < b.Length && 0 <= l < i + j ==> b[k] >= c[l]
+    {
+        if i < a.Length && (j == b.Length || a[i] <= b[j]) {
+            c[i + j] := a[i];
+            i := i + 1;
+        }
+        else {
+            c[i + j] := b[j];
+            j := j + 1;
+        }
+    }
+}
+
+method testMerge() {
+    var a: array<T> := new T[3] [1, 3, 5];
+    var b: array<T> := new T[2] [2, 4];
+    var c:= merge(a, b);
+    assert a[..a.Length] == [1, 3, 5];
+    assert b[..b.Length] == [2, 4];
+    assert elems(c, c.Length) == multiset{1, 2, 3, 4, 5};
+    assert c[..] == [1, 2, 3, 4, 5];
+}
