Testes anteriores/T2/ex7_2020.dfy
@@ -1,0 +1,32 @@
+type T = int
+
+class {:autocontracts} BSTNode {
+    // Concrete implementation variables.
+    var value: T 
+    var left: BSTNode?  // elements smaller than 'value' (? - may be null)
+    var right: BSTNode? // elements greater than 'value' (? - may be null)
+
+    // Ghost variable used for specification & verification purposes.
+    // Holds the set of values in the subtree starting in this node (inclusive). 
+    ghost var elems: set<T> 
+
+    // Class invariant with the integrity constraints for the above variables
+    predicate Valid() 
+        reads this
+    { 
+        (this.elems == {value} + (if left != null then left.elems else {}) + (if right != null then right.elems else {})) &&
+        (left != null ==> forall x :: x in left.elems ==> x < value) &&
+        (right != null ==> forall x :: x in right.elems ==> x > value)
+    }
+
+    // Check if the subtree starting in this node contains a value 'x'.
+    method contains(x: T) returns (res: bool)
+      ensures res <==> x in elems
+      decreases elems
+    {
+        if x == value { res := true; } 
+        else if x < value && left != null  { res := left.contains(x); } 
+        else if x > value && right != null { res := right.contains(x); } 
+        else { res := false; }
+    }
+}
