Testes anteriores/T2/ex7_2020_2.dfy
@@ -1,0 +1,35 @@
+class {:autocontracts} Customer { }
+class {:autocontracts} Book {
+    const id: nat;
+    var holder: Customer?; // current rental holder of the book, or null
+    var queue: seq<Customer>; // list of customers with pending rental requests,
+                            // by temporal order (oldest request at position 0)
+
+    /* Class invariant */
+    predicate Valid() // a)
+        reads this
+    {
+        (holder != null ==> holder !in queue) &&
+        forall i, j :: 0 <= i < j < |queue| ==> queue[i] != queue[j]
+
+    }
+    /* Operations */
+    constructor (id: nat)
+    method pickBook(customer: Customer) // b)
+        requires holder == null
+        requires (|queue| > 0 && queue[0] == customer) || |queue| == 0
+        ensures holder == customer
+        ensures queue == old(if queue == [] then queue else queue[1..])
+    {
+
+    }
+     
+    method reserveBook(customer: Customer)
+    method returnBook(customer: Customer)
+    method cancelReservation(customer: Customer) // c)
+        requires customer in queue && |queue| > 0
+        ensures customer !in queue && |queue| == old(|queue|) - 1 
+    {
+
+    }
+}
