Testes anteriores/T2/factorial.dfy
@@ -1,0 +1,28 @@
+function method fact(n: nat) : nat
+    decreases n
+{
+    if n == 0 then 1 else n * fact(n-1)
+}
+
+method factIter(n: nat) returns (f : nat)
+    requires n >= 0
+    ensures f == fact(n)
+{
+    f := 1;
+    var i := 0;
+    while i < n
+        decreases n - i
+        invariant 0 <= i <= n && fact(i) == f
+    {
+        i := i + 1;
+        f := f * i;
+    }
+}
+
+method Main()
+{
+    var f := 6;
+    var x := factIter(f);
+    print "fact(", f, ") = ", x, "\n";
+    assert x == 720;
+}
