Testes anteriores/T2/fibonacci.dfy
@@ -1,0 +1,20 @@
+function fib(n : nat ) : nat
+    decreases n
+{
+    if n < 2 then n else fib(n - 2) + fib(n - 1)
+}
+
+method computeFib (n : nat) returns (x : nat)
+    ensures x == fib(n)
+{
+    var i := 0;
+    x := 0;
+    var y := 1;
+    while i < n
+        invariant fib(i) == x && fib(i + 1) == y && 0 <= i <= n
+        decreases n - i
+    {
+        x, y := y, x + y; // multiple assignment
+        i := i + 1;
+    }
+}
