Testes anteriores/T2/person.dfy
@@ -1,0 +1,112 @@
+datatype Sex = Masculine | Feminine
+datatype CivilState = Single | Married | Divorced | Widow | Dead
+
+class Person
+{
+    const name: string; // ‘const’ for immutable fields
+    const sex: Sex;
+    const mother: Person?; // ‘?’ to allow null
+    const father: Person?;
+    var spouse: Person?;
+    var civilState: CivilState;
+    ghost const ancestors : set<Person>
+
+    constructor (name: string, sex: Sex, mother: Person?, father: Person?)
+        requires (mother != null ==> mother.sex == Feminine)
+        requires (father != null ==> father.sex == Masculine)
+        ensures this.name == name 
+        ensures this.sex == sex 
+        ensures this.mother == mother 
+        ensures this.father == father 
+        ensures this.spouse == null 
+        ensures this.civilState == Single
+        ensures this.ancestors == (if this.mother != null then {this.mother} + this.mother.ancestors else {}) + (if this.father != null then {this.father} + this.father.ancestors else {})
+        ensures Valid()
+    {
+        this.name := name;
+        this.sex := sex;
+        this.mother := mother;
+        this.father := father;
+        this.spouse := null;
+        this.civilState := Single;
+        this.ancestors := (if mother != null then {mother} + mother.ancestors else {}) + (if father != null then {father} + father.ancestors else {});
+    }
+
+    predicate Valid() 
+        reads this, spouse
+    {
+        (this.spouse != null <==> this.civilState == Married) &&
+        (this.mother != null ==> this.mother.sex == Feminine) &&
+        (this.father != null ==> this.father.sex == Masculine) &&
+        (this.spouse != null ==> this.spouse.spouse == this && this.spouse.sex != this.sex && this.spouse !in ancestors && (this.spouse.father != null ==> spouse.father != this.father) && (this.spouse.mother != null ==> spouse.mother != this.mother)) &&
+        (ancestors == (if this.mother != null then {this.mother} + this.mother.ancestors else {}) + (if this.father != null then {this.father} + this.father.ancestors else {}))
+    }
+
+    method marry(spouse: Person)
+        modifies this, spouse
+        requires Valid()
+        requires this.civilState != Married && this.civilState != Dead
+        requires spouse.civilState != Married && spouse.civilState != Dead
+        requires this.sex != spouse.sex
+        requires spouse !in ancestors && this !in spouse.ancestors
+        requires spouse.father != null ==> this.father != spouse.father 
+        requires spouse.mother != null ==> this.mother != spouse.mother
+        ensures Valid()
+        ensures this.spouse == spouse
+        ensures this.civilState == Married
+        ensures spouse.civilState == Married
+        ensures spouse.spouse == this
+    {
+        spouse.spouse := this;
+        spouse.civilState := Married;
+        this.spouse := spouse;
+        this.civilState := Married;
+    }
+
+    method divorce()
+        modifies this, spouse
+        requires Valid()
+        requires civilState == Married
+        ensures Valid()
+        ensures old(spouse).spouse == null
+        ensures old(spouse).civilState == Divorced
+        ensures this.spouse == null
+        ensures this.civilState == Divorced
+    {
+        spouse.civilState := Divorced;
+        spouse.spouse := null;
+        this.spouse := null;
+        this.civilState := Divorced;
+    }
+
+    method die()
+        modifies this, spouse
+        requires Valid()
+        requires this.civilState != Dead
+        ensures Valid()
+        ensures (old(spouse) != null ==> old(spouse).civilState == Widow && old(spouse).spouse == null)
+        ensures this.spouse == null
+        ensures this.civilState == Dead
+    {
+        if spouse != null
+        {
+            spouse.civilState := Widow;
+            spouse.spouse := null;
+        }
+        this.spouse := null;
+        this.civilState := Dead;
+    }
+}
+
+// Test scenario to cover all valid transitions of civil state (checking post-conditions).
+method Main()
+{
+    var person := new Person("vitor", Masculine, null, null);
+    var person2 := new Person("catarina", Feminine, null, null);
+
+    person.marry(person2);
+
+    assert person.spouse == person2;
+    assert person2.spouse == person;
+    assert person.sex != person2.sex;
+}
