Testes anteriores/T2/hoare_logic.md
@@ -1,0 +1,206 @@
+# Exercises on Program Verification with Hoare Logic
+
+## Exercise 1
+
+**a)** True
+
+**b)** False
+
+**c)** True
+
+**d)** True
+
+**e)** True
+
+## Exercise 2
+
+**a)**
+
+```
+wp(S,Q)
+= wp(x := x+1, x > 5)
+= x + 1 > 5
+= x > 4
+```
+
+**b)**
+
+```
+wp(S,Q)
+= wp(if a>b then x:=a else x:=b, x > 0)
+= (a>b ∧ wp(x:=a, x>0)) ∨ (a<=b ∧ wp(x:=b, x>0))
+= (a>b ∧ a>0) ∨ (a<=b ∧ b>0)
+= a>0 ∨ b>0
+```
+
+**c)** wp(S,Q) = x>=y
+
+## Exercise 3
+
+**a)**
+
+```
+wp(skip, x>0)
+= x>0
+
+P -> wp(S,Q)
+<=> x>5 -> x>0
+<=> True
+```
+
+**b)**
+
+```
+wp(x:=x+1, x>5)
+= x+1 > 5
+= x > 4
+
+P -> wp(S,Q)
+<=> x<6 -> x>4
+<=> x>=6 ∨ x>4
+<=> x>4
+
+Since this does not reduce to true (does not always hold), the triple is not valid
+```
+
+**c)**
+
+```
+wp(if x>0 then y:=10 else skip, y=10)
+= (x>0 ∧ wp(y:=10, y=10)) ∨ (x<=0 ∧ wp(skip, y=10))
+= (x>0 ∧ (10=10)) ∨ (x<=0 ∧ y=10)
+= x>0 ∨ (x<=0 ∧ y=10)
+= x>0 ∨ y=10
+
+P -> wp(S,Q)
+<=> (x=5 ∧ y=0) -> x>0 ∨ y=10
+<=> True
+```
+
+**d)**
+
+```
+wp(x:=y, y:=a; x=b ∧ y=a)
+= wp(x:=y, wp(y:=a; x=b ∧ y=a))
+= wp(x:=y, x=b ∧ a=a)
+= wp(x:=y, x=b)
+= y = b
+
+P -> wp(S,Q)
+<=> (x=a ∧ y=b) -> y=b
+<=> True
+```
+
+## Exercise 4
+
+```
+P -> I
+<=> x > y -> x >= y
+<=> True
+
+I ∧ ¬C -> Q
+<=> (x >= y) ∧ (x <= y) -> x = y
+<=> x = y => x = y
+<=> True
+
+{I ∧ C ∧ V = V0}S{I ∧ 0 <= V < V0}
+<=> {(x >= y) ∧ (x > y) ∧ (x-y = V0)} x:=x-1 {(x >= y) ∧ 0 <= x-y <= V0}
+<=> {x > y ∧ x-y=V0} x:=x-1 {x >= y ∧ x-y < V0}
+<=> (x > y ∧ x-y=V0) => (x-1 >= y ∧ x-1-y < V0)
+<=> (x > y ∧ x-y=V0) => (x >= y+1 ∧ x-y <= V0)
+<=> (x>y ∧ x-y=V0) => (x > y ∧ x-y <= V0)
+<=> True
+
+So the given triple is Valid
+```
+
+## Exercise 5
+
+```
+// Identify loop invariants and variants
+I = r >= 0 ∧ d > 0 ∧ q * d + r = D
+V = r
+
+// Insert loop variants and invariants
+{D >= 0 ∧ d > 0}
+q := 0;
+r := D;
+**{r >= 0 ∧ d > 0 ∧ q * d + r = D} // I**
+while r >= d do
+    **{r >= 0 ∧ d > 0 ∧ q * d + r = D ∧ r >= d ∧ r = V0} // I ∧ C ∧ V = V0**
+    q := q + 1;
+    r := r - d;
+    **{r >= 0 ∧ d > 0 ∧ q * d + r = D ∧ 0 <= V < V0} // I ∧ 0 <= V < V0**
+** {r >= 0 ∧ d > 0 ∧ q * d + r = D ∧ r < d} // I ∧ ¬C
+{0 <= r < d ∧ q * d + r = D}
+
+// Calculate pre-conditions bottom-up
+{D >= 0 ∧ d > 0}
+***{D >= 0 ∧ d > 0 ∧ 0 * d + D = D}***
+q := 0;
+***{D >= 0 ∧ d > 0 ∧ q * d + D = D}***
+r := D;
+**{r >= 0 ∧ d > 0 ∧ q * d + r = D} // I**
+while r >= d do
+    **{r >= 0 ∧ d > 0 ∧ q * d + r = D ∧ r >= d ∧ r = V0} // I ∧ C ∧ V = V0**
+    ***{r-d >= 0 ∧ d > 0 ∧ (q+1) * d + (r-d) = D ∧ 0 <= r-d < V0}***
+    q := q + 1;
+    ***{r-d >= 0 ∧ d > 0 ∧ q * d + (r-d) = D ∧ 0 <= r-d < V0}***
+    r := r - d;
+    **{r >= 0 ∧ d > 0 ∧ q * d + r = D ∧ 0 <= V < V0} // I ∧ 0 <= V < V0**
+** {r >= 0 ∧ d > 0 ∧ q * d + r = D ∧ r < d} // I ∧ ¬C
+{0 <= r < d ∧ q * d + r = D}
+
+// Prove implications of consecutive conditions
+(D >= 0 ∧ d > 0 => D >= 0 ∧ d > 0 ∧ 0 * d + D = D)
+<=> (D >= 0 ∧ d > 0 => D >= 0 ∧ d > 0 ∧ D = D)
+<=> (D >= 0 ∧ d > 0 => D >= 0 ∧ d > 0)
+<=> True
+
+(r >= 0 ∧ d > 0 ∧ q * d + r = D ∧ r >= d ∧ r = V0 => r-d >= 0 ∧ d > 0 ∧ (q+1) * d + (r-d) = D ∧ 0 <= r-d < V0)
+<=> (d > 0 ∧ q * d + r = D ∧ r >= d ∧ r = V0 ==> r >= d ∧ d > 0 ∧ q * d + r = D ∧ r < V0 + d)
+<=> True
+
+(r >= 0 ∧ d > 0 ∧ q * d + r = D ∧ r < d => 0 <= r < d ∧ q * d + r = D)
+<=> (r >= 0 ∧ d > 0 ∧ q * d + r = D ∧ r < d => r >= 0 ∧ d > 0 ∧ q * d + r = D)
+<=> True
+```
+
+## Exercise 6
+
+**a)**
+
+```
+{x >= 0}
+**{x >= 0}**
+z := x;
+**{z + 0 = x ∧ z >= 0}**
+y := 0;
+{z + y = x ∧ z >= 0} //I
+while z != 0 do
+    {z != 0 ∧ z + y = x ∧ z >= 0 ∧ z = V0} // C ∧ I ∧ V = V0
+    **{z + y = x ∧ z - 1 >= 0 ∧ 0 <= z - 1 < V0}**
+    y := y + 1
+    **{z - 1 + y = x ∧ z - 1 >= 0 ∧ 0 <= z - 1 < V0}**
+    z := z - 1;
+    {z + y = x ∧ z >= 0 ∧ 0 <= z < V0} // I ∧ 0 <= V < V0
+{z = 0 ∧ z + y = x ∧ z >= 0} // ¬C ∧ I
+{x = y}
+```
+
+**b)**
+
+```
+(x >= 0 => x >= 0) <=> True
+
+(z != 0 ∧ z + y = x ∧ z >= 0 ∧ z = V0 => z + y = x ∧ z - 1 >= 0 ∧ 0 <= z - 1 < V0)
+<=> (z + y = x ∧ z > 0 ∧ z = V0 => z + y = x ∧ z > 0 ∧ z - 1 < V0)
+<=> (z + y = x ∧ z > 0 ∧ z = V0 => z + y = x ∧ z > 0 ∧ V0 - 1 < V0)
+<=> (z + y = x ∧ z > 0 ∧ z = V0 => z + y = x ∧ z > 0)
+<=> True
+
+(z = 0 ∧ z + y = x ∧ z >= 0 => x = y)
+<=> (z = 0 ∧ z + y = x => x = y)
+<=> (y = x => x = y)
+<=> True
+```
